chore: Converted copy decreases examples

examples/copyDecreasesBenchmarks/formula.dfy
@@ -1,26 +1,49 @@
-import benchmarks_formula_defs._
-import stainless.lang._
+datatype Formula = 
+  True_
+  | False_
+  | Not(param0: Formula)
+  | AndAlso(param0: Formula, param1: Formula)
+  | OrElse(param0: Formula, param1: Formula)
+  | Imply(param0: Formula, param1: Formula)
+  | Equal(left: Exp, right: Exp)
 
-object C_formula_sol359 {
-   
-  
-  def evall(e: Exp): Int = {
-    e match {
-      case Num(a) => { a }
-      case Plus(a, b) => { evall(a) + evall(b) }
-      case Minus(a, b) => { evall(a) - evall(b) }
-    }
+datatype Exp = Num(num: int) | Plus(param0: Exp, param1: Exp) | Minus(param0: Exp, param1: Exp)
+
+function size(f: Formula): int
+  ensures size(f) >= 0
+{
+  match f {
+    case True_ => 0
+    case False_ => 0
+    case Not(p) => 1 + size(p)
+    case AndAlso(p0, p1) => 2 + size(p0) + size(p1)
+    case OrElse(p0, p1) => 2 + size(p0) + size(p1)
+    case Imply(p0, p1) => 10 + size(p0) + size(p1)
+    case Equal(_, _) => 1
   }
-  
-  def eval(f: Formula): Boolean = {
-    f match {
-      case True_ => { true }
-      case False_ => { false }
-      case Not(a) => { if (eval(a)) false else true }
-      case AndAlso(a, b) => { eval(a) && eval(b) }
-      case OrElse(a, b) => { eval(a) || eval(b) }
-      case Imply(a, b) => { eval(Not(AndAlso(a, Not(b)))) }
-      case Equal(a, b) => { if (evall(a) == evall(b)) true else false }
-    }
+}
+
+function evall(e: Exp): int {
+  match e {
+    case Num(a) => a
+    case Plus(a, b) => evall(a) + evall(b)
+    case Minus(a, b) => evall(a) - evall(b)
+  }
+}
+
+// The termination clause here needed to be manually put in
+function eval(f: Formula): bool
+  decreases size(f)
+{
+  match f {
+    case True_ => true
+    case False_ => false
+    case Not(a) => if (eval(a)) then false else true
+    case AndAlso(a, b) => eval(a) && eval(b)
+    case OrElse(a, b) => eval(a) || eval(b)
+    case Imply(a, b) =>
+      assert size(Not(AndAlso(a, Not(b)))) < size(Imply(a, b));
+      eval(Not(AndAlso(a, Not(b))))
+    case Equal(a, b) => if (evall(a) == evall(b)) then true else false
   }
 }
