examples/copyDecreasesBenchmarks/refs/formula.dfy
@@ -1,38 +1,56 @@
-import stainless.lang._
-import benchmarks_formula_defs._
+datatype Formula = 
+  True_
+  | False_
+  | Not(param0: Formula)
+  | AndAlso(param0: Formula, param1: Formula)
+  | OrElse(param0: Formula, param1: Formula)
+  | Imply(param0: Formula, param1: Formula)
+  | Equal(left: Exp, right: Exp)
 
-object ta_solutions_formula_solution {
+datatype Exp = Num(num: int) | Plus(param0: Exp, param1: Exp) | Minus(param0: Exp, param1: Exp)
 
-object ta_solutions_formula {
-  def evalM(f: Formula): Boolean = {
-    decreases(f.size)
-    f match {
-      case True_ => { true }
-      case False_ => { false }
-      case Not(f) => !(evalM(f))
-      case AndAlso(p1, p2) =>
-        lazy val p11 = evalM(p1)
-        lazy val p22 = evalM(p2)
-        p11 && p22
-      case OrElse(p1, p2) =>
-        lazy val p11 = evalM(p1)
-        lazy val p22 = evalM(p2)
-        p11 || p22
-      case Imply(p1, p2)  =>
-        lazy val p11 = evalM(p1)
-        lazy val p22 = evalM(p2)
-        !(p11) || p22
-      case Equal(p1, p2) =>
-        def exp_evalM(exp: Exp): Int = {
-          exp match {
-            case Num(n) => { n }
-            case Plus(e1, e2) => { exp_evalM(e1) + exp_evalM(e2) }
-            case Minus(e1, e2) => { exp_evalM(e1) - exp_evalM(e2) }
-          }
-        }
-        exp_evalM(p1) == exp_evalM(p2)
-    }
+function size(f: Formula): int
+  ensures size(f) >= 0
+{
+  match f {
+    case True_ => 0
+    case False_ => 0
+    case Not(p) => 1 + size(p)
+    case AndAlso(p0, p1) => 2 + size(p0) + size(p1)
+    case OrElse(p0, p1) => 2 + size(p0) + size(p1)
+    case Imply(p0, p1) => 10 + size(p0) + size(p1)
+    case Equal(_, _) => 1
   }
 }
 
+function exp_evalM(exp: Exp): int {
+  match exp {
+    case Num(n) => n
+    case Plus(e1, e2) => exp_evalM(e1) + exp_evalM(e2)
+    case Minus(e1, e2) => exp_evalM(e1) - exp_evalM(e2)
+  }
+}
+
+function evalM(f: Formula): bool
+  decreases(size(f))
+{
+  match f {
+    case True_ => true
+    case False_ => false
+    case Not(f) => !(evalM(f))
+    case AndAlso(p1, p2) =>
+      var p11 := evalM(p1);
+      var p22 := evalM(p2);
+      p11 && p22
+    case OrElse(p1, p2) =>
+      var p11 := evalM(p1);
+      var p22 := evalM(p2);
+      p11 || p22
+    case Imply(p1, p2)  =>
+      var p11 := evalM(p1);
+      var p22 := evalM(p2);
+      !(p11) || p22
+    case Equal(p1, p2) =>
+      exp_evalM(p1) == exp_evalM(p2)
+  }
 }
