examples/copyDecreasesBenchmarks/refs/prime.dfy
@@ -1,51 +1,77 @@
-package s12
 
 /* Copyright 2022 EPFL, Lausanne */
 
-import stainless.lang._
 
 // ./stainless ../evaluation/Prime.scala --timeout=2 --solvers=smt-z3 --equivchk=true --models=isPrimeM --comparefuns=isPrime  --vc-cache=false
 // source: epfl softcon 2023
 
-object Prime:
+function recM(n: int, i: int): int
+  requires(n >= 0 && i > 0 && i-1 <= n)
+  decreases(n-i+1)
+  ensures recM(n, i) >= 0 // Added this line
+{
+  if i == n / i then i
+  else if i > n / i then i - 1
+  else recM(n, i+1)
+}
 
-  def isqrtM(n: BigInt): BigInt =
-    require(n >= 0)
-    def recM(n: BigInt, i: BigInt): BigInt =
-      require(n >= 0 && i > 0 && i-1 <= n)
-      decreases(n-i+1)
-      if i == n / i then i
-      else if i > n / i then i - 1
-      else recM(n, i+1)
-    recM(n, 1)
+function isqrtM(n: int): int
+  requires(n >= 0)
+{
+  recM(n, 1)
+}
 
-  def isPrimeM1(n: BigInt): Boolean =
-    require(n >= 0)
-    def innerM1(k: BigInt, ref: BigInt): Boolean =
-      require(k > 0 && ref > 0 && ref <= k)
-      decreases(k-ref)
-      if ref > Prime.isqrtM(k) then
-        true
-      else
-        if k%ref == 0 then
-          false
-        else
-          innerM1(k, ref+1)
-    if n <= 1 then
+function innerM1(k: int, ref: int): bool
+  requires(k > 0 && ref > 0 && ref <= k)
+  decreases(k-ref)
+{
+  if ref > isqrtM(k) then
+    true
+  else
+    if k%ref == 0 then
       false
     else
-      innerM1(n, 2)
+      innerM1(k, ref+1)
+}
 
-  def isPrimeM2(n: BigInt): Boolean =
-    require(n >= 0)
-    def innterM2(n: BigInt, i: BigInt): Boolean =
-      require(n >= 0 && i > 1 && i <= n)
-      decreases(n-i)
-      if (i >= n) then true
-      else if (n % i == 0) then false
-      else innterM2(n, i + 1)
+function isPrimeM1(n: int): bool
+  requires(n >= 0)
+{
+  if n <= 1 then
+    false
+  else
+    innerM1(n, 2)
+}
 
-    if (n == 0 || n == 1) then
-      false
-    else
-      innterM2(n, 2)
+function innterM2(n: int, i: int): bool
+  requires(n >= 0 && i > 1 && i <= n)
+  decreases(n-i)
+{
+  if (i >= n) then true
+  else if (n % i == 0) then false
+  else innterM2(n, i + 1)
+}
+
+function isPrimeM2(n: int): bool
+  requires(n >= 0)
+{
+  if (n == 0 || n == 1) then
+    false
+  else
+    innterM2(n, 2)
+}
+
+function isPrimeHelperC(n: int, i: int): bool
+  requires i >= 0 // Added this line
+  decreases i // Added this line
+{
+  if i == 1 || i == 0 then true 
+  else n%i != 0 && isPrimeHelperC(n, i-1)
+}
+
+function isPrimeC(n: int): bool 
+  requires(n >= 0)
+{
+  if n == 0 || n == 1 then false 
+  else isPrimeHelperC(n, isqrtM(n))
+}
