examples/copyDecreasesBenchmarks/gcd.dfy
@@ -1,16 +1,10 @@
-package s13
 
-object s13_04f3cfaef7c4d9d49a7d26f5bd84ed7e:
-
-  /** @param a
-    *   A natural number
-    * @param b
-    *   A natural number
-    * @return
-    *   Int : The greatest common divisor between a and b
-    */
-  def gcd(a: Int, b: Int): Int =
-    require(a >= 0 && b >= 0)
-    if b == 0 then a
-    else if a < b then gcd(b,a)
-    else gcd(b, a % b)
+// The decreases clause needed to be added here
+function gcd(a: int, b: int): int
+  requires(a >= 0 && b >= 0)
+  decreases b
+{
+  if b == 0 then a
+  else if a < b then gcd(b,a)
+  else gcd(b, a % b)
+}
