examples/copyDecreasesBenchmarks/refs/gcd.dfy
@@ -1,32 +1,31 @@
 /* Copyright 2022 EPFL, Lausanne */
-
-import stainless.lang._
-
 // source: epfl softcon 2023
 
-object GCD:
-
-  def gcdM1(a: Int, b: Int): Int =
-    require(a >= 0 && b >= 0)
-    decreases(a, b)
-    if a == b then 
-      a
-    else
-      if a > b then 
-        if b == 0 then 
-          a
-        else
-          gcdM1(a - b, b)
+function gcdM1(a: int, b: int): int
+  requires (a >= 0 && b >= 0)
+  decreases a, b
+{
+  if a == b then 
+    a
+  else
+    if a > b then 
+      if b == 0 then 
+        a
       else
-        if a == 0 then
-          b
-        else
-          gcdM1(a, b - a)
-
-  def gcdM2(a: Int, b: Int): Int =
-    require(a >= 0 && b >= 0)
-    decreases(a/2 + b/2 + (if(b-a >=2) (b-a)/2 else if(b-a >= 0) (b-a+2)/2 else 0))
-    if b == 0 then
-      a
+        gcdM1(a - b, b)
     else
-      gcdM2(b, a%b)
+      if a == 0 then
+        b
+      else
+        gcdM1(a, b - a)
+}
+
+function gcdM2(a: int, b: int): int
+  requires (a >= 0 && b >= 0)
+  decreases(a/2 + b/2 + (if (b-a >=2) then (b-a)/2 else if (b-a >= 0) then (b-a+2)/2 else 0))
+  {
+  if b == 0 then
+    a
+  else
+    gcdM2(b, a%b)
+  }
