examples/copyDecreasesBenchmarks/refs/sigma.dfy
@@ -1,31 +1,30 @@
-import stainless.collection._
-import stainless.lang._
-object ta_solutions_sigma {
-  def solution_1(f: BigInt => BigInt, a: BigInt, b: BigInt): BigInt = {
-    decreases(if (b == a) BigInt(2) else if (b > a) 2 + b - a else a - b)
-    if (a > b) {
-      BigInt(0)
-    } else if (a == b) {
-      f(a)
-    } else {
-      f(a) + solution_1(f, a + BigInt(1), b)
-    }
-  }
-  def solution_2(f: BigInt => BigInt, a: BigInt, b: BigInt): BigInt = {
-    decreases(if (b == a) BigInt(2) else if (b > a) 2 + b - a else a - b)
-    if (a > b) {
-      BigInt(0)
-    } else if (a == b) {
-      f(a)
-    } else {
-      f(b) + solution_2(f, a, b - BigInt(1))
-    }
-  }
-  def solution_3(f: BigInt => BigInt, a: BigInt, b: BigInt): BigInt = {
-    def s(a: BigInt, b: BigInt, f: BigInt => BigInt, acc: BigInt): BigInt = {
-      decreases(if (b == a) BigInt(2) else if (b > a) 2 + b - a else a - b)
-      if (a > b) acc else s(a + BigInt(1), b, f, acc + f(a))
-    }
-    s(a, b, f, BigInt(0))
-  }
+function solution_1(f: int -> int, a: int, b: int): int
+  decreases(if (b == a) then 2 else if (b > a) then 2 + b - a else a - b)
+{
+  if (a > b) then
+    0
+  else if (a == b) then
+    f(a)
+  else
+    f(a) + solution_1(f, a + 1, b)
+}
+function solution_2(f: int -> int, a: int, b: int): int
+  decreases(if (b == a) then 2 else if (b > a) then 2 + b - a else a - b)
+{
+  if (a > b) then
+    0
+  else if (a == b) then
+    f(a)
+  else
+    f(b) + solution_2(f, a, b - 1)
+}
+
+function s(a: int, b: int, f: int -> int, acc: int): int
+  decreases(if (b == a) then 2 else if (b > a) then 2 + b - a else a - b)
+{
+  if (a > b) then acc else s(a + 1, b, f, acc + f(a))
+}
+
+function solution_3(f: int -> int, a: int, b: int): int {
+  s(a, b, f, 0)
 }
